don't define the access using the heap explicitely

Weidenbach_Book/Array_Array_List.thy
@@ -14,98 +14,96 @@ lemma heap_list_add_same_length:
   \<open>h \<Turnstile> heap_list_all R' xs p \<Longrightarrow> length p = length xs\<close>
   by (induction R' xs p arbitrary: h rule: heap_list_all.induct) (auto elim!: mod_starE)
 
-definition nth_aa :: "'a::heap array_list array \<Rightarrow> nat \<Rightarrow> nat \<Rightarrow> 'a Heap" where
-  [code del]: "nth_aa a i j = Heap_Monad.guard (\<lambda>h. i < Array.length h a \<and> j < snd (Array.get h a ! i))
-    (\<lambda>h. (Array.get h (fst (Array.get h a ! i)) ! j, h))"
-
-lemma run_nth_aa[run_elims]:
-  assumes "run (nth_aa a i j) \<sigma> \<sigma>' r"
-          "\<not>is_exn \<sigma>"
-  obtains "\<not>is_exn \<sigma>"
-    "i < Array.length (the_state \<sigma>) a"
-    "r = (Array.get (the_state \<sigma>) (fst ((Array.get (the_state \<sigma>) a)! i))) ! j"
-    "j < snd ((Array.get (the_state \<sigma>) a)! i)"
-    "\<sigma>' = \<sigma>"
-  |
-    "\<not> i < Array.length (the_state \<sigma>) a"
-    "\<sigma>' = None"
-  |
-    "\<not>j < snd ((Array.get (the_state \<sigma>) a)! i)"
-    "\<sigma>' = None"
-  using assms
-  apply (cases \<sigma>)
-   apply (solves \<open>simp\<close>)
-  apply (cases "\<not>i < Array.length (the_state \<sigma>) a")
-   apply (solves \<open>simp add: run.simps nth_aa_def execute_guard(1)\<close>)
-  apply (cases "\<not>j < snd ((Array.get (the_state \<sigma>) a)! i)")
-   apply (solves \<open>simp add: run.simps nth_aa_def execute_guard(1)\<close>)
-  by (auto simp add: run.simps nth_aa_def execute_guard)
+definition nth_aa where
+  \<open>nth_aa xs i j = do {
+      x \<leftarrow> Array.nth xs i;
+      y \<leftarrow> arl_get x j;
+      return y}\<close>
 
 lemma models_heap_list_all_models_nth:
   \<open>(h, as) \<Turnstile> heap_list_all R a b \<Longrightarrow> i < length a \<Longrightarrow> \<exists>as'. (h, as') \<Turnstile> R (a!i) (b!i)\<close>
   by (induction R a b arbitrary: as i rule: heap_list_all.induct)
     (auto simp: mod_star_conv nth_Cons elim!: less_SucE split: nat.splits)
 
-lemma nth_aa:
-  assumes
-    i: \<open>i < length xs\<close> and j: \<open>j < length (xs ! i)\<close> and p: \<open>is_pure R'\<close>
+definition nth_ll :: "'a list list \<Rightarrow> nat \<Rightarrow> nat \<Rightarrow> 'a" where
+  \<open>nth_ll l i j = l ! i ! j\<close>
+
+lemma nth_aa_hnr[sepref_fr_rules]:
+  assumes p: \<open>is_pure R\<close>
   shows
-    \<open><arrayO (arl_assn R') xs a> nth_aa a i j <\<lambda>r. arrayO (arl_assn R') xs a * R' (xs ! i ! j) r>\<^sub>t\<close>
+    \<open>(uncurry2 nth_aa, uncurry2 (RETURN \<circ>\<circ>\<circ> nth_ll)) \<in>
+     [\<lambda>((l,i),j). i < length l \<and> j < length (l ! i)]\<^sub>a (arrayO (arl_assn R))\<^sup>k *\<^sub>a nat_assn\<^sup>k *\<^sub>a nat_assn\<^sup>k \<rightarrow> R\<close>
 proof -
-  obtain R where R: \<open>the_pure R' = R\<close> and R': \<open>R' = pure R\<close>
+  obtain R' where R: \<open>the_pure R = R'\<close> and R': \<open>R = pure R'\<close>
     using p by fastforce
+  have [simp]: \<open>(\<exists>\<^sub>Ax. arrayO (arl_assn R) a ai * R x r * true * \<up> (x = a ! ba ! b)) =
+     (arrayO (arl_assn R) a ai * R (a ! ba ! b) r * true)\<close> for a ai ba b r
+    by (auto simp: ex_assn_def)
   show ?thesis
-    unfolding nth_aa_def
-    unfolding hoare_triple_def snga_assn_def array_assn_def is_array_def nth_aa_def
-  proof (clarsimp simp only: Let_def Abs_assn_inverse, intro allI impI conjI)
-    fix h :: Heap.heap and as :: \<open>nat set\<close> and \<sigma> :: \<open>Heap.heap option\<close> and
-      r :: 'b
+  proof (sepref_to_hoare, clarsimp simp only: hoare_triple_def Let_def, intro allI impI conjI)
+    fix a :: \<open>'a list list\<close> and ai :: \<open>('b array_list) array\<close> and
+      h :: Heap.heap and as:: \<open>nat set\<close> and \<sigma> :: \<open>Heap.heap option\<close> and r :: 'b and
+      i i' j j' :: nat
     assume
-      h: \<open>(h, as) \<Turnstile> arrayO (arl_assn R') xs a\<close> and
-      run: \<open>run (Heap_Monad.guard (\<lambda>h. i < Array.length h a \<and> j < snd (Array.get h a ! i)) 
-          (\<lambda>h. (Array.get h (fst (Array.get h a ! i)) ! j, h))) (Some h) \<sigma> r\<close>
-    have [simp]: \<open>i < Array.length h a\<close>
+      i: \<open>i < length a\<close> and
+      j: \<open>j < length (a ! i)\<close> and
+      h: \<open> (h, as) \<Turnstile>
+       \<up> ((j', j) \<in> nat_rel) * \<up> ((i', i) \<in> nat_rel) *
+       arrayO (arl_assn R) a ai\<close> and
+      run: \<open>run (nth_aa ai i' j') (Some h) \<sigma> r\<close>
+
+    have i_le: \<open>i < Array.length h ai\<close>
       using h i unfolding arrayO_def array_assn_def is_array_def
       by (auto simp: run.simps tap_def arrayO_def
           mod_star_conv array_assn_def is_array_def
           Abs_assn_inverse heap_list_add_same_length length_def snga_assn_def)
-    have xs_i: \<open>\<exists>as'. (h, as') \<Turnstile> (arl_assn R') (xs ! i) ((Array.get h a ! i))\<close>
+    have xs_i: \<open>\<exists>as'. (h, as') \<Turnstile> (arl_assn R) (a ! i) (Array.get h ai ! i)\<close>
       using h i unfolding arrayO_def array_assn_def is_array_def
       using models_heap_list_all_models_nth[of _ _ _ _ _ i]
       by (auto simp: run.simps tap_def arrayO_def
           mod_star_conv array_assn_def is_array_def
           Abs_assn_inverse heap_list_add_same_length length_def snga_assn_def)
-    then have j_le_get[simp]: \<open>j < snd (Array.get h a ! i)\<close>
+    then have j_le_get: \<open>j < Array.length h (fst (Array.get h ai ! i))\<close>
       using j unfolding arrayO_def arl_assn_def is_array_list_def
-      by (cases \<open>Array.get h a ! i\<close>) (auto simp: run.simps tap_def arrayO_def hr_comp_def
+      by (cases \<open>Array.get h ai ! i\<close>) (auto simp: run.simps tap_def arrayO_def hr_comp_def
           mod_star_conv array_assn_def is_array_def
           Abs_assn_inverse heap_list_add_same_length length_def snga_assn_def
           dest: list_rel_pres_length)
-
+    have j_le_get_snd: \<open>j < snd (Array.get h ai ! i)\<close>
+      using j xs_i unfolding arrayO_def arl_assn_def is_array_list_def
+      by (cases \<open>Array.get h ai ! i\<close>) (auto simp: run.simps tap_def arrayO_def hr_comp_def
+          mod_star_conv array_assn_def is_array_def
+          Abs_assn_inverse heap_list_add_same_length length_def snga_assn_def
+          dest: list_rel_pres_length)
+    have ex_arl: \<open>execute (arl_get (Array.get h ai ! i) j) h =
+        Some (Array.get h (fst (Array.get h ai ! i)) ! j, h)\<close>
+      using run h assms i_le i j j_le_get
+      by (auto simp: run.simps tap_def arrayO_def execute_simps
+          mod_star_conv array_assn_def is_array_def nth_aa_def Array.nth_def
+          Abs_assn_inverse heap_list_add_same_length snga_assn_def
+          execute_bind_case arl_get_def split_beta
+          split: option.splits)
+    have ex: \<open>execute (nth_aa ai i j) h = Some (Array.get h (fst (Array.get h ai ! i)) ! j, h)\<close>
+      using run h assms i_le
+      by (auto simp: run.simps tap_def arrayO_def execute_simps ex_arl
+          mod_star_conv array_assn_def is_array_def nth_aa_def Array.nth_def
+          Abs_assn_inverse heap_list_add_same_length length_def snga_assn_def
+          execute_bind_case split: option.splits)
     show \<open>\<not> is_exn \<sigma>\<close>
       using run h assms
-      by (auto simp: run.simps tap_def arrayO_def execute_simps
-          mod_star_conv array_assn_def is_array_def
-          Abs_assn_inverse heap_list_add_same_length length_def snga_assn_def)
-    have ex: \<open>execute
-        (Heap_Monad.guard
-          (\<lambda>h. i < length (Array.get h a) \<and>
-               j < snd (Array.get h a ! i))
-          (\<lambda>h. (Array.get h (fst (Array.get h a ! i)) ! j, h)))
-        h = Some (Array.get h (fst (Array.get h a ! i)) ! j, h)\<close>
-      using run h assms
-      by (auto simp: run.simps tap_def arrayO_def execute_simps
-          mod_star_conv array_assn_def is_array_def
+      by (auto simp: run.simps tap_def arrayO_def execute_simps ex
+          mod_star_conv array_assn_def is_array_def Array.nth_def
           Abs_assn_inverse heap_list_add_same_length length_def snga_assn_def)
     show \<open>(the_state \<sigma>, new_addrs h as (the_state \<sigma>)) \<Turnstile>
-       arrayO (arl_assn R') xs a  * R' (xs ! i ! j) r * true\<close>
-      using run h assms xs_i j_le_get
-      apply (cases \<open>Array.get h a ! i\<close>) 
-      apply (auto simp: run.simps tap_def arrayO_def R R'
+       \<up> ((j', j) \<in> nat_rel) * \<up> ((i', i) \<in> nat_rel) * arrayO (arl_assn R) a ai *
+            (\<exists>\<^sub>Ax. R x r * \<up> (RETURN x \<le> RETURN (nth_ll a i j))) * true\<close>
+      using run h assms xs_i j_le_get i_le j_le_get_snd
+      apply (cases \<open>Array.get h ai ! i\<close>)
+      apply (auto simp: run.simps tap_def arrayO_def R R' nth_ll_def
           mod_star_conv arl_assn_def is_array_list_def hr_comp_def ex list_rel_def
           Abs_assn_inverse heap_list_add_same_length length_def snga_assn_def
-          dest!: list_all2_nthD[of _ _ _ j] simp del: j_le_get)
-      by blast -- \<open>TODO well tune proof\<close>
+          dest!: list_all2_nthD[of _ _ _ j])
+        by blast
     show \<open>relH {a. a < lim h \<and> a \<notin> as} h (the_state \<sigma>)\<close>
       using run h assms xs_i
       by (auto simp: run.simps tap_def arrayO_def
@@ -121,24 +119,6 @@ proof -
   qed
 qed
 
-definition nth_ll :: "'a list list \<Rightarrow> nat \<Rightarrow> nat \<Rightarrow> 'a" where
-  \<open>nth_ll l i j = l ! i ! j\<close>
-  
-lemma [sepref_fr_rules]:
-  assumes \<open>is_pure R\<close>
-  shows
-    \<open>(uncurry2 nth_aa, uncurry2 (RETURN \<circ>\<circ>\<circ> nth_ll)) \<in>
-     [\<lambda>((l,i),j). i < length l \<and> j < length (l ! i)]\<^sub>a (arrayO (arl_assn R))\<^sup>k *\<^sub>a nat_assn\<^sup>k *\<^sub>a nat_assn\<^sup>k \<rightarrow> R\<close>
-proof -
-  have [simp]: \<open>(\<exists>\<^sub>Ax. arrayO (arl_assn R) a ai * R x r * true * \<up> (x = a ! ba ! b)) =
-     (arrayO (arl_assn R) a ai * R (a ! ba ! b) r * true)\<close> for a ai ba b r
-    by (auto simp: ex_assn_def)
-  show ?thesis
-    using assms
-    apply sepref_to_hoare
-    by (auto simp: nth_ll_def nth_aa IS_PURE_def)
-qed
-  
 definition update_aa where
   \<open>update_aa a i x = Array.upd a i x\<close>
 
@@ -147,11 +127,15 @@ term Array.update
 term \<open>Array.set a (list_update (Array.get h a) i x) h\<close>
 term arl_assn
 term arl_append
-definition arl_append_heap where
-"arl_append_heap \<equiv> \<lambda>a i x.
-  let j = Array.nth a i in
-  let a' = arl_append j x in
-  a'"
+
+definition append_el_aa where
+"append_el_aa \<equiv> \<lambda>a i x. do {
+  j \<leftarrow> Array.nth a i;
+  a' \<leftarrow> arl_append j x;
+  Array.upd i a' a
+  }"
+
+
 
 definition append_aa :: "'a::heap array_list array \<Rightarrow> nat \<Rightarrow> 'a \<Rightarrow> 'a Heap" where
   [code del]: "append_aa a i x = Heap_Monad.guard (\<lambda>h::Heap.heap. i < Array.length h a \<and> j < snd (Array.get h a ! i))
